@prefix : <https://imagoarchive.it/ontology/> .
@prefix owl: <http://www.w3.org/2002/07/owl#> .
@prefix rdf: <http://www.w3.org/1999/02/22-rdf-syntax-ns#> .
@prefix xml: <http://www.w3.org/XML/1998/namespace> .
@prefix xsd: <http://www.w3.org/2001/XMLSchema#> .
@prefix foaf: <http://xmlns.com/foaf/0.1/> .
@prefix rdfs: <http://www.w3.org/2000/01/rdf-schema#> .
@prefix skos: <http://www.w3.org/2004/02/skos/core#> .
@prefix vann: <http://purl.org/vocab/vann/> .
@prefix dcterms: <http://purl.org/dc/terms/> .
@base <http://www.w3.org/2002/07/owl#> .

[ rdf:type owl:Ontology ;
   owl:imports <http://imagoarchive.it/ilrmoo/> ,
               <https://imagoarchive.it/thes/tid/> ;
   dcterms:contributor "Emanuele Lenzi" ,
                       "Irene Parlanti" ;
   dcterms:creator <https://www.isti.cnr.it/en/about/people-detail/38/Valentina_Bartalesi_Lenzi> ,
                   <https://www.isti.cnr.it/en/about/people-detail/820/Nicol%C3%B2_Pratelli> ;
   dcterms:description "The IMAGO ontology provides elements of description for  Middle Ages and Renaissance manuscripts and printed edition, in particular those defined in the IMAGO project."@en ;
   dcterms:issued "2021-07-12" ;
   dcterms:modified "2022-11-22" ;
   dcterms:publisher <https://www.isti.cnr.it/> ;
   dcterms:title "The IMAGO Ontology" ;
   vann:preferredNamespacePrefix "imago" ;
   vann:preferredNamespaceUri : ;
   rdfs:comment """Modifications from version 0.1:
          Deleted: Pubblication Place Appellation, is composed of place name
          Modified: unnecessary axioms in many classes"""@en ;
   rdfs:isDefinedBy :imago-221122.ttl ;
   owl:Import <http://imagoarchive.it/ilrmoo/> ;
   owl:priorVersion <https://imagoarchive.it/onto/imago-220930.ttl> ;
   foaf:homepage <https://imagoarchive.it/documentation/doc/index-en.html>
 ] .

#################################################################
#    Annotation properties
#################################################################

###  http://purl.org/dc/terms/contributor
dcterms:contributor rdf:type owl:AnnotationProperty .


###  http://purl.org/dc/terms/creator
dcterms:creator rdf:type owl:AnnotationProperty .


###  http://purl.org/dc/terms/description
dcterms:description rdf:type owl:AnnotationProperty .


###  http://purl.org/dc/terms/issued
dcterms:issued rdf:type owl:AnnotationProperty .


###  http://purl.org/dc/terms/modified
dcterms:modified rdf:type owl:AnnotationProperty .


###  http://purl.org/dc/terms/publisher
dcterms:publisher rdf:type owl:AnnotationProperty .


###  http://purl.org/dc/terms/title
dcterms:title rdf:type owl:AnnotationProperty .


###  http://purl.org/vocab/vann/preferredNamespacePrefix
vann:preferredNamespacePrefix rdf:type owl:AnnotationProperty .


###  http://purl.org/vocab/vann/preferredNamespaceUri
vann:preferredNamespaceUri rdf:type owl:AnnotationProperty .


###  http://www.w3.org/2002/07/owl#Import
owl:Import rdf:type owl:AnnotationProperty .


###  http://xmlns.com/foaf/0.1/homepage
foaf:homepage rdf:type owl:AnnotationProperty .


###  http://xmlns.com/foaf/0.1/workplaceHomepage
foaf:workplaceHomepage rdf:type owl:AnnotationProperty .


#################################################################
#    Object Properties
#################################################################

###  http://erlangen-crm.org/211015/P14_carried_out_by
<http://erlangen-crm.org/211015/P14_carried_out_by> rdf:type owl:ObjectProperty .


###  http://erlangen-crm.org/211015/P1_is_identified_by
<http://erlangen-crm.org/211015/P1_is_identified_by> rdf:type owl:ObjectProperty .


###  http://erlangen-crm.org/211015/P50_has_current_keeper
<http://erlangen-crm.org/211015/P50_has_current_keeper> rdf:type owl:ObjectProperty .


###  http://erlangen-crm.org/211015/P74_has_current_or_former_residence
<http://erlangen-crm.org/211015/P74_has_current_or_former_residence> rdf:type owl:ObjectProperty .


###  https://imagoarchive.it/ontology/has_curator
:has_curator rdf:type owl:ObjectProperty ;
             rdfs:subPropertyOf <http://erlangen-crm.org/211015/P14_carried_out_by> ;
             rdfs:domain <http://imagoarchive.it/ilrmoo/F30_Manifestation_Creation> ;
             rdfs:range :Curator ;
             rdfs:comment "In the IMAGO Ontology 'has curator' links a F30 Manifestation Creation to a Curator"@en ;
             rdfs:label "has curator"@en .


###  https://imagoarchive.it/ontology/has_genre
:has_genre rdf:type owl:ObjectProperty ;
           rdfs:subPropertyOf <http://erlangen-crm.org/211015/P2_has_type> ;
           rdfs:domain <http://imagoarchive.it/ilrmoo/F2_Expression> ;
           rdfs:range :Genre ;
           rdfs:comment "In the IMAGO Ontology property hasGenre links F2 Expression to class Genre."@en ;
           rdfs:label "has genre"@en .


###  https://imagoarchive.it/ontology/has_publisher
:has_publisher rdf:type owl:ObjectProperty ;
               rdfs:subPropertyOf <http://erlangen-crm.org/211015/P14_carried_out_by> ;
               rdfs:domain <http://imagoarchive.it/ilrmoo/F30_Manifestation_Creation> ;
               rdfs:range :Publisher ;
               rdfs:comment "In the IMAGO Ontology 'has publisher' links a F30 Manifestation Creation to a Publisher"@en ;
               rdfs:label "has publisher"@en .


###  https://imagoarchive.it/ontology/is_explicit_dedication
:is_explicit_dedication rdf:type owl:ObjectProperty ;
                        rdfs:subPropertyOf <http://erlangen-crm.org/211015/P106i_forms_part_of> ;
                        rdfs:domain <http://erlangen-crm.org/211015/E90_Symbolic_Object> ;
                        rdfs:range <http://imagoarchive.it/ilrmoo/F3_Manifestation> ;
                        rdfs:comment "In the IMAGO Ontology 'is explicit dedication of' links E90 Symbolic Object to Manuscript class"@en ;
                        rdfs:label "is explicit dedication of"@en .


###  https://imagoarchive.it/ontology/is_identified_by_toponym
:is_identified_by_toponym rdf:type owl:ObjectProperty ;
                          rdfs:subPropertyOf <http://erlangen-crm.org/211015/P1_is_identified_by> ;
                          rdfs:domain <http://erlangen-crm.org/211015/E53_Place> ;
                          rdfs:range :Toponym ;
                          rdfs:comment "In the IMAGO Ontology is identified by toponym relates a place to its toponym."@en ;
                          rdfs:label "is identified by toponym"@en .


###  https://imagoarchive.it/ontology/is_identified_in_the_printed_edition_by
:is_identified_in_the_printed_edition_by rdf:type owl:ObjectProperty ;
                                         rdfs:subPropertyOf <http://erlangen-crm.org/211015/P1_is_identified_by> ;
                                         rdfs:domain <http://erlangen-crm.org/211015/E53_Place> ;
                                         rdfs:range <http://erlangen-crm.org/211015/E41_Appellation> ;
                                         rdfs:comment "In the IMAGO Ontology is identified in the printed edition by links E53 Place to E41 Appellation, hence a place to the name it is identified by in a printed edition."@en ;
                                         rdfs:label "is identified in the printed edition by"@en .


###  https://imagoarchive.it/ontology/is_incipit_dedication_of
:is_incipit_dedication_of rdf:type owl:ObjectProperty ;
                          rdfs:subPropertyOf <http://erlangen-crm.org/211015/P106i_forms_part_of> ;
                          rdfs:domain <http://erlangen-crm.org/211015/E90_Symbolic_Object> ;
                          rdfs:range <http://imagoarchive.it/ilrmoo/F3_Manifestation> ;
                          rdfs:comment "In the IMAGO Ontology 'is incipit dedication of' links E90 Symbolic Object to class Manuscript"@en ;
                          rdfs:label "is incipit dedication of"@en .


###  https://imagoarchive.it/ontology/is_text_explicit_of
:is_text_explicit_of rdf:type owl:ObjectProperty ;
                     rdfs:subPropertyOf <http://erlangen-crm.org/211015/P106i_forms_part_of> ;
                     rdfs:domain <http://erlangen-crm.org/211015/E90_Symbolic_Object> ;
                     rdfs:range <http://imagoarchive.it/ilrmoo/F3_Manifestation> ;
                     rdfs:comment "In the IMAGO Ontology 'is text explicit of' links E90 Symbolic Object to class Manuscript"@en ;
                     rdfs:label "is text explicit of"@en .


###  https://imagoarchive.it/ontology/is_text_incipit_of
:is_text_incipit_of rdf:type owl:ObjectProperty ;
                    rdfs:subPropertyOf <http://erlangen-crm.org/211015/P106i_forms_part_of> ;
                    rdfs:domain <http://erlangen-crm.org/211015/E90_Symbolic_Object> ;
                    rdfs:range <http://imagoarchive.it/ilrmoo/F3_Manifestation> ;
                    rdfs:comment "In the IMAGO Ontology 'is text incipit of' links E90 Symbolic Object to class Manuscript"@en ;
                    rdfs:label "is text incipit of"@en .


#################################################################
#    Data properties
#################################################################

###  http://erlangen-crm.org/211015/P190_has_symbolic_content
<http://erlangen-crm.org/211015/P190_has_symbolic_content> rdf:type owl:DatatypeProperty .


###  http://xmlns.com/foaf/0.1/name
foaf:name rdf:type owl:DatatypeProperty .


###  https://imagoarchive.it/ontology/has_VDL_explanation
:has_VDL_explanation rdf:type owl:DatatypeProperty ;
                     rdfs:domain :Toponym ;
                     rdfs:range xsd:string ;
                     rdfs:label "has VDL explanation"@en .


###  https://imagoarchive.it/ontology/has_figure_note
:has_figure_note rdf:type owl:DatatypeProperty ;
                 rdfs:subPropertyOf <http://erlangen-crm.org/211015/P3_has_note> ;
                 rdfs:domain :Printed_Edition ;
                 rdfs:range xsd:string ;
                 rdfs:comment "In the IMAGO Ontology 'has figure note' links Print Edition to a literal (string) in order to express knowledge about figures in the print edition"@en ;
                 rdfs:label "has figure note"@en .


###  https://imagoarchive.it/ontology/has_genre_name
:has_genre_name rdf:type owl:DatatypeProperty ;
                rdfs:domain :Genre ;
                rdfs:range xsd:string ;
                rdfs:comment "In the IMAGO Ontology has genre name links tha class Genre to the corresponding literal (a string)."@en ;
                rdfs:label "has genre name"@en .


###  https://imagoarchive.it/ontology/has_iconographic_apparatus
:has_iconographic_apparatus rdf:type owl:DatatypeProperty ;
                            rdfs:subPropertyOf <http://erlangen-crm.org/211015/P3_has_note> ;
                            rdfs:domain :Manuscript ;
                            rdfs:range xsd:string ;
                            rdfs:comment "In the IMAGO Ontology has iconographic apparatus links Manuscript to a literal ( a string) in order to express knowledge about the iconographic apparatus of a manuscript."@en ;
                            rdfs:label "has iconographic apparatus"@en .


###  https://imagoarchive.it/ontology/has_introduction_note
:has_introduction_note rdf:type owl:DatatypeProperty ;
                       rdfs:subPropertyOf <http://erlangen-crm.org/211015/P3_has_note> ;
                       rdfs:domain :Printed_Edition ;
                       rdfs:range xsd:string ;
                       rdfs:comment "In the IMAGO Ontology has introduction note links Print Edition to a literal (string) in order to express knowledge about the author of the introduction and dedications in a print edition"@en ;
                       rdfs:label "has introduction note"@en .


###  https://imagoarchive.it/ontology/has_other_contents
:has_other_contents rdf:type owl:DatatypeProperty ;
                    rdfs:subPropertyOf <http://erlangen-crm.org/211015/P3_has_note> ;
                    rdfs:domain :Printed_Edition ;
                    rdfs:range xsd:string ;
                    rdfs:comment "In the IMAGO Ontology 'has other contents' links Print Edition to a literal (string) in order to express knowledge about other contents in the print edition"@en ;
                    rdfs:label "has other contents"@en .


###  https://imagoarchive.it/ontology/has_primary_source
:has_primary_source rdf:type owl:DatatypeProperty ;
                    rdfs:subPropertyOf <http://erlangen-crm.org/211015/P3_has_note> ;
                    rdfs:domain <http://erlangen-crm.org/211015/E1_CRM_Entity> ;
                    rdfs:range xsd:string ;
                    rdfs:comment "In the IMAGO Ontology 'has primary source' links Print Edition to a literal (string) in order to express knowledge about primary sources in the print edition"@en ;
                    rdfs:label "has primary source"@en .


###  https://imagoarchive.it/ontology/has_reprint_date
:has_reprint_date rdf:type owl:DatatypeProperty ;
                  rdfs:subPropertyOf <http://erlangen-crm.org/211015/P3_has_note> ;
                  rdfs:domain <http://erlangen-crm.org/211015/E1_CRM_Entity> ;
                  rdfs:range xsd:string ;
                  rdfs:comment "In the IMAGO Ontology 'has reprint date' links Print Edition to a literal (string) in order to express knowledge about the date of reprints, facsimile or anastatic edition in the print edition"@en ;
                  rdfs:label "has reprint date"@en .


###  https://imagoarchive.it/ontology/has_secondary_source
:has_secondary_source rdf:type owl:DatatypeProperty ;
                      rdfs:subPropertyOf <http://erlangen-crm.org/211015/P3_has_note> ;
                      rdfs:domain <http://erlangen-crm.org/211015/E1_CRM_Entity> ;
                      rdfs:range xsd:string ;
                      rdfs:comment "In the IMAGO Ontology 'has figure note' links Print Edition to a literal (string) in order to express knowledge about figures in the print edition and manuscript"@en ;
                      rdfs:label "has secondary source"@en .


###  https://imagoarchive.it/ontology/has_textual_place
:has_textual_place rdf:type owl:DatatypeProperty ;
                   rdfs:subPropertyOf owl:topDataProperty ;
                   rdfs:domain <http://erlangen-crm.org/211015/E90_Symbolic_Object> ;
                   rdfs:range xsd:string ;
                   rdfs:label "has textual place"@en .


###  https://imagoarchive.it/ontology/has_url_manuscript
:has_url_manuscript rdf:type owl:DatatypeProperty ;
                    rdfs:subPropertyOf <http://erlangen-crm.org/211015/P3_has_note> ;
                    rdfs:domain :Manuscript ;
                    rdfs:range xsd:string ;
                    rdfs:comment "In the IMAGO Ontology 'has url manuscript' links Manuscript to a literal (anyURI) in order to express the URI of the digital representation of the manuscript"@en ;
                    rdfs:label "has url manuscript"@en .


###  https://imagoarchive.it/ontology/has_url_manuscript_description
:has_url_manuscript_description rdf:type owl:DatatypeProperty ;
                                rdfs:subPropertyOf <http://erlangen-crm.org/211015/P3_has_note> ;
                                rdfs:domain :Manuscript ;
                                rdfs:range xsd:string ;
                                rdfs:comment "In the IMAGO Ontology 'has url manuscript description' links Manuscript to a literal (anyURI) in order to express the URI of the digital description of the manuscript"@en ;
                                rdfs:label "has url manuscript description"@en .


#################################################################
#    Classes
#################################################################

###  http://erlangen-crm.org/211015/E19_Physical_Object
<http://erlangen-crm.org/211015/E19_Physical_Object> rdf:type owl:Class .


###  http://erlangen-crm.org/211015/E41_Appellation
<http://erlangen-crm.org/211015/E41_Appellation> rdfs:subClassOf [ rdf:type owl:Restriction ;
                                                                   owl:onProperty <http://erlangen-crm.org/211015/P190_has_symbolic_content> ;
                                                                   owl:someValuesFrom xsd:string
                                                                 ] .


###  http://erlangen-crm.org/211015/E42_Identifier
<http://erlangen-crm.org/211015/E42_Identifier> rdf:type owl:Class ;
                                                rdfs:subClassOf [ rdf:type owl:Restriction ;
                                                                  owl:onProperty <http://erlangen-crm.org/211015/P190_has_symbolic_content> ;
                                                                  owl:someValuesFrom xsd:string
                                                                ] .


###  http://erlangen-crm.org/211015/E53_Place
<http://erlangen-crm.org/211015/E53_Place> rdf:type owl:Class .


###  http://erlangen-crm.org/211015/E90_Symbolic_Object
<http://erlangen-crm.org/211015/E90_Symbolic_Object> rdfs:subClassOf [ rdf:type owl:Restriction ;
                                                                       owl:onProperty <http://erlangen-crm.org/211015/P190_has_symbolic_content> ;
                                                                       owl:someValuesFrom xsd:string
                                                                     ] .


###  http://imagoarchive.it/ilrmoo/F28_Expression_Creation
<http://imagoarchive.it/ilrmoo/F28_Expression_Creation> rdfs:subClassOf [ rdf:type owl:Restriction ;
                                                                          owl:onProperty <http://erlangen-crm.org/211015/P14_carried_out_by> ;
                                                                          owl:someValuesFrom :Author
                                                                        ] ,
                                                                        [ rdf:type owl:Restriction ;
                                                                          owl:onProperty <http://imagoarchive.it/ilrmoo/R17_created> ;
                                                                          owl:someValuesFrom <http://imagoarchive.it/ilrmoo/F2_Expression>
                                                                        ] .


###  http://imagoarchive.it/ilrmoo/F30_Manifestation_Creation
<http://imagoarchive.it/ilrmoo/F30_Manifestation_Creation> rdfs:subClassOf [ rdf:type owl:Restriction ;
                                                                             owl:onProperty <http://imagoarchive.it/ilrmoo/R24_created> ;
                                                                             owl:someValuesFrom <http://imagoarchive.it/ilrmoo/F3_Manifestation>
                                                                           ] .


###  http://imagoarchive.it/ilrmoo/F3_Manifestation
<http://imagoarchive.it/ilrmoo/F3_Manifestation> rdfs:subClassOf [ rdf:type owl:Restriction ;
                                                                   owl:onProperty <http://imagoarchive.it/ilrmoo/R4_embodies> ;
                                                                   owl:someValuesFrom <http://imagoarchive.it/ilrmoo/F2_Expression>
                                                                 ] .


###  http://xmlns.com/foaf/0.1/Organization
foaf:Organization rdf:type owl:Class .


###  http://xmlns.com/foaf/0.1/Person
foaf:Person rdf:type owl:Class .


###  https://imagoarchive.it/ontology/Author
:Author rdf:type owl:Class ;
        rdfs:subClassOf <http://erlangen-crm.org/211015/E39_Actor> ,
                        [ rdf:type owl:Restriction ;
                          owl:onProperty <http://erlangen-crm.org/211015/P1_is_identified_by> ;
                          owl:someValuesFrom <http://erlangen-crm.org/211015/E41_Appellation>
                        ] ;
        rdfs:comment "In the IMAGO Ontology class Author represents one of the main categories of the conceptualization, the Author."@en ;
        rdfs:label "Author"@en .


###  https://imagoarchive.it/ontology/Curator
:Curator rdf:type owl:Class ;
         rdfs:subClassOf <http://erlangen-crm.org/211015/E39_Actor> ,
                         [ rdf:type owl:Restriction ;
                           owl:onProperty <http://erlangen-crm.org/211015/P1_is_identified_by> ;
                           owl:someValuesFrom <http://erlangen-crm.org/211015/E41_Appellation>
                         ] ;
         rdfs:comment "In the IMAGO Ontology Curator class expresses knowledge about the curator of a printed edition."@en ;
         rdfs:label "Curator"@en .


###  https://imagoarchive.it/ontology/Edition
:Edition rdf:type owl:Class ;
         rdfs:subClassOf <http://erlangen-crm.org/211015/E55_Type> ;
         rdfs:comment "In the IMAGO Ontology Edition is defined in order to express knowledge about first editions or reprinted editions"@en ;
         rdfs:label "Edition"@en .


###  https://imagoarchive.it/ontology/Folios
:Folios rdf:type owl:Class ;
        rdfs:subClassOf <http://erlangen-crm.org/211015/E19_Physical_Object> ,
                        [ rdf:type owl:Restriction ;
                          owl:onProperty <http://erlangen-crm.org/211015/P1_is_identified_by> ;
                          owl:someValuesFrom <http://erlangen-crm.org/211015/E41_Appellation>
                        ] ;
        rdfs:comment "In the IMAGO Ontology class Folios is used to represent the folios of a manuscript."@en ;
        rdfs:label "Folios"@en .


###  https://imagoarchive.it/ontology/Format
:Format rdf:type owl:Class ;
        rdfs:subClassOf <http://erlangen-crm.org/211015/E55_Type> ,
                        [ rdf:type owl:Restriction ;
                          owl:onProperty <http://erlangen-crm.org/211015/P1_is_identified_by> ;
                          owl:someValuesFrom <http://erlangen-crm.org/211015/E41_Appellation>
                        ] ;
        rdfs:comment "In the IMAGO Ontology Format class expresses knowledge about the format of a printed edition."@en ;
        rdfs:label "Format"@en .


###  https://imagoarchive.it/ontology/Genre
:Genre rdf:type owl:Class ;
       rdfs:subClassOf <http://erlangen-crm.org/211015/E55_Type> ,
                       [ rdf:type owl:Restriction ;
                         owl:onProperty :has_genre_name ;
                         owl:someValuesFrom xsd:string
                       ] ;
       rdfs:comment "In the IMAGO Ontology the Genre class represents the literary genre of a F2 Expression, namely a work."@en ;
       rdfs:label "Genre"@en .


###  https://imagoarchive.it/ontology/Library
:Library rdf:type owl:Class ;
         rdfs:subClassOf <http://imagoarchive.it/ilrmoo/F11_Corporate_Body> ,
                         [ rdf:type owl:Restriction ;
                           owl:onProperty <http://erlangen-crm.org/211015/P74_has_current_or_former_residence> ;
                           owl:someValuesFrom <http://erlangen-crm.org/211015/E53_Place>
                         ] ;
         rdfs:comment "In the IMAGO Ontology class Library represents the library where a manuscript is stored."@en ;
         rdfs:label "Library"@en .


###  https://imagoarchive.it/ontology/Manuscript
:Manuscript rdf:type owl:Class ;
            rdfs:subClassOf <http://imagoarchive.it/ilrmoo/F5_Item> ,
                            [ rdf:type owl:Restriction ;
                              owl:onProperty <http://erlangen-crm.org/211015/P1_is_identified_by> ;
                              owl:someValuesFrom <http://erlangen-crm.org/211015/E42_Identifier>
                            ] ,
                            [ rdf:type owl:Restriction ;
                              owl:onProperty <http://erlangen-crm.org/211015/P50_has_current_keeper> ;
                              owl:someValuesFrom :Library
                            ] ,
                            [ rdf:type owl:Restriction ;
                              owl:onProperty <http://imagoarchive.it/ilrmoo/R7_is_materialization_of> ;
                              owl:someValuesFrom <http://imagoarchive.it/ilrmoo/F3_Manifestation>
                            ] ;
            rdfs:comment "In the IMAGO Ontology class Manuscript represents a kind of resource, the manuscript of a work."@en ;
            rdfs:label "Manuscript"@en .


###  https://imagoarchive.it/ontology/Printed_Edition
:Printed_Edition rdf:type owl:Class ;
                 rdfs:subClassOf <http://imagoarchive.it/ilrmoo/F3_Manifestation> ;
                 rdfs:comment "In the IMAGO Ontology class Printed Edition represents a kind of resource, the printed edition of a work."@en ;
                 rdfs:label "Printed Edition"@en .


###  https://imagoarchive.it/ontology/Publisher
:Publisher rdf:type owl:Class ;
           rdfs:subClassOf <http://erlangen-crm.org/211015/E39_Actor> ,
                           [ rdf:type owl:Restriction ;
                             owl:onProperty <http://erlangen-crm.org/211015/P1_is_identified_by> ;
                             owl:someValuesFrom <http://erlangen-crm.org/211015/E41_Appellation>
                           ] ;
           rdfs:comment "In the IMAGO Ontology Publisher class expresses knowledge about the editor/publisher of a printed edition."@en ;
           rdfs:label "Publisher"@en .


###  https://imagoarchive.it/ontology/Toponym
:Toponym rdf:type owl:Class ;
         rdfs:subClassOf <http://erlangen-crm.org/211015/E41_Appellation> ;
         rdfs:comment "In the IMAGO Ontology Toponym class is defined as a subclass of CRM E41 Appellation class to represents toponyms."@en ;
         rdfs:label "Toponym"@en .


###  https://imagoarchive.it/ontology/Typology
:Typology rdf:type owl:Class ;
          rdfs:subClassOf <http://erlangen-crm.org/211015/E55_Type> ;
          rdfs:comment "In the IMAGO Ontology Typology is defined in order to express knowledge about ecdotic typology"@en ;
          rdfs:label "Typology"@en .


#################################################################
#    Individuals
#################################################################

###  https://www.isti.cnr.it/
<https://www.isti.cnr.it/> rdf:type owl:NamedIndividual ,
                                    foaf:Organization ;
                           rdfs:label "ISTI-CNR" ;
                           foaf:homepage <https://www.isti.cnr.it/en/> .


###  https://www.isti.cnr.it/en/about/people-detail/38/Valentina_Bartalesi_Lenzi
<https://www.isti.cnr.it/en/about/people-detail/38/Valentina_Bartalesi_Lenzi> rdf:type owl:NamedIndividual ,
                                                                                       foaf:Person ;
                                                                              foaf:name "Valentina Bartalesi Lenzi" ;
                                                                              rdfs:label "Valentina Bartalesi" ;
                                                                              foaf:workplaceHomepage <https://www.isti.cnr.it/en/> .


###  https://www.isti.cnr.it/en/about/people-detail/820/Nicol%C3%B2_Pratelli
<https://www.isti.cnr.it/en/about/people-detail/820/Nicol%C3%B2_Pratelli> rdf:type owl:NamedIndividual ,
                                                                                   foaf:Person ;
                                                                          foaf:name "Nicolò Pratelli" ;
                                                                          rdfs:label "Nicolò Pratelli" ;
                                                                          foaf:workplaceHomepage <https://www.isti.cnr.it/en/> .


###  Generated by the OWL API (version 4.5.9.2019-02-01T07:24:44Z) https://github.com/owlcs/owlapi
